src/coq/Handlers/MemoryModel.v
@@ -3,6 +3,7 @@ From Vellvm.Syntax Require Import
      DynamicTypes.
 
 From Vellvm.Semantics Require Import
+     MemoryAddress
      MemoryParams
      LLVMParams
      LLVMEvents.
@@ -27,37 +28,46 @@ From Coq Require Import
      ZArith.
 
 Import Basics.Basics.Monads.
+Import MonadNotation.
+Open Scope monad_scope.
+
+(* Move this ? *)
+Definition store_id := N.
+Class MonadStoreID (M : Type -> Type) : Type :=
+  { fresh_sid : M store_id;
+    get_sid : M store_id;
+    put_sid : store_id -> M unit;
+  }.
+
+Class MonadMemState (MemState : Type) (M : Type -> Type) : Type :=
+  { get_mem_state : M MemState;
+    put_mem_state : MemState -> M unit;
+  }.
+
+Definition modify_mem_state {M MemState} `{Monad M} `{MonadMemState MemState M} (f : MemState -> MemState) : M MemState :=
+  ms <- get_mem_state;;
+  put_mem_state (f ms);;
+  ret ms.
+
+(* TODO: Add RAISE_PICK or something... May need to be in a module *)
+Class MemMonad (MemState : Type) (Provenance : Type) (M : Type -> Type)
+      `{Monad M}
+      `{MonadProvenance Provenance M} `{MonadStoreID M} `{MonadMemState MemState M}
+      `{RAISE_ERROR M} `{RAISE_UB M} `{RAISE_OOM M} : Type
+  :=
+  { MemMonad_runs_to {A} (ma : M A) (ms : MemState) : option (MemState * A);
+    MemMonad_lift_stateT
+      {E} `{FailureE -< E} `{UBE -< E} `{OOME -< E} {A}
+      (ma : M A) : stateT MemState (itree E) A;
+  }.
 
 (* Module types for memory models to allow different memory models to be plugged in. *)
 Module Type MemoryModel (LP : LLVMParams) (MP : MemoryParams LP).
   Import LP.Events.
   Import LP.ADDR.
+  Import LP.SIZEOF.
 
-  (* TODO: Clean up / move this stuff *)
   Import LP.PROV.
-  Parameter store_id : Type.
-
-  Class MonadProvenance (M : Type -> Type) : Type :=
-    { fresh_provenance : M Provenance
-    }.
-
-  Class MonadStoreID (M : Type -> Type) : Type :=
-    { fresh_sid : M store_id
-    }.
-
-  Class MonadMemState (MemState : Type) (M : Type -> Type) : Type :=
-    { get_mem_state : M MemState;
-      put_mem_state : MemState -> M unit
-    }.
-
-
-  Class MemMonad (MemState : Type) (M : Type -> Type)
-        `{MonadProvenance M} `{MonadStoreID M} `{MonadMemState MemState M}
-        `{RAISE_ERROR M} `{RAISE_UB M} `{RAISE_OOM M} : Type
-    :=
-    { MemMonad_runs_to {A} (ma : M A) (ms : MemState) : option (MemState * A);
-    }.
-
   (* TODO: Should DataLayout be here? 
 
      It might make sense to move DataLayout to another module, some of
@@ -67,49 +77,114 @@ Module Type MemoryModel (LP : LLVMParams) (MP : MemoryParams LP).
      For instance alignment may impact Sizeof, and there's also some
      stuff about pointer sizes in the DataLayout structure.
    *)
-  Parameter datalayout : DataLayout.
+  (* Parameter datalayout : DataLayout. *)
 
   (** Datatype for the state of memory *)
   Parameter MemState : Type.
   Parameter initial_memory_state : MemState.
 
+  Definition MemStateT := stateT MemState.
+
+  Instance MemStateT_MonadProvenance {M} :
+    MonadProvenance Provenance (MemStateT M).
+  Proof.
+  Admitted.
+
+  Instance MemStateT_MonadStoreID {M} :
+    MonadStoreID (MemStateT M).
+  Proof.
+  Admitted.
+
+  Instance MemStateT_MonadMemState {M} :
+    MonadMemState MemState (MemStateT M).
+  Proof.
+    split.
+    eapply (MonadState.get).
+    eapply (MonadState.put).
+  Admitted.
+
+  Parameter free_concrete_space :
+    forall (ms : MemState) (phys_addr : Z) (sz : N), bool.
+
+  Definition concrete_memory_pick_post
+             (st : MemState * (addr * dtyp)) (phys_addr : Z) : Prop
+    := match st with
+       | (ms, (a, dt)) =>
+           free_concrete_space ms phys_addr (sizeof_dtyp dt) = true
+       end.
+
+  Definition PickConcreteMemoryE :=
+    @PickE (MemState * (addr * dtyp)) Z concrete_memory_pick_post.
+
+  (* Not sure if we need this yet *)
+  Parameter free_logical_space :
+    forall (ms : MemState) (ptr : addr) (sz : N), bool.
+
+  Definition PickLogicalMemoryE :=
+    @PickE (MemState * dtyp) addr
+           (fun '(ms, dt) ptr =>
+              free_logical_space ms ptr (sizeof_dtyp dt) = true).
+
+  Instance MemStateT_itree_MemMonad
+           {E} `{FailureE -< E} `{UBE -< E} `{OOME -< E} `{PickConcreteMemoryE -< E}
+    : MemMonad MemState Provenance (MemStateT (itree E)).
+  Admitted.
+
+  (* (** MemMonad *) *)
+  (* Parameter MemMonad : Type -> Type. *)
+
+  (* (** Extra monad classes *) *)
+  (* Parameter MemMonad_MonadStoreID : MonadStoreID MemMonad. *)
+  (* Parameter MemMonad_MonadProvenance : MonadProvenance Provenance MemMonad. *)
+  (* Parameter MemMonad_MonadMemState : MonadMemState MemState MemMonad. *)
+
+  (* Parameter MemMonad_RAISE_ERROR : RAISE_ERROR MemMonad. *)
+  (* Parameter MemMonad_RAISE_UB : RAISE_UB MemMonad. *)
+  (* Parameter MemMonad_RAISE_OOM : RAISE_OOM MemMonad. *)
+  (* Parameter MemMonad_RAISE_PICK : RAISE_PICK MemMonad. *)
+
+  (* (* Hack to make typeclass resolution work... *) *)
+  (* Hint Resolve MemMonad_MonadStoreID : typeclass_instances. *)
+  (* Hint Resolve MemMonad_MonadProvenance : typeclass_instances. *)
+  (* Hint Resolve MemMonad_MonadMemState : typeclass_instances. *)
+  (* Hint Resolve MemMonad_RAISE_ERROR : typeclass_instances. *)
+  (* Hint Resolve MemMonad_RAISE_UB : typeclass_instances. *)
+  (* Hint Resolve MemMonad_RAISE_OOM : typeclass_instances. *)
+  (* Hint Resolve MemMonad_RAISE_PICK : typeclass_instances. *)
+
+  (* Parameter MemMonad_runs_to : forall {A} (ma : MemMonad A) (ms : MemState), option (MemState * A). *)
+  (* Parameter MemMonad_lift_stateT :  *)
+  (*   forall {E} `{FailureE -< E} `{UBE -< E} `{OOME -< E} `{PickE -< E} {A} *)
+  (*     (ma : MemMonad A), stateT MemState (itree E) A. *)
+
   (** Basic operations on the state of logical memory. *)
   Parameter allocate :
-    forall {M : Type -> Type}
-      `{MemMonad MemState M},
-      dtyp -> M addr.
+    forall {M} `{MemMonad MemState Provenance M} (dt : dtyp),
+      M addr.
 
   Parameter allocated :
-    forall {M : Type -> Type}
-      `{MemMonad MemState M}
-      (ptr : addr),
+    forall {M} `{MemMonad MemState Provenance M} (ptr : addr),
       M bool.
 
   Parameter read :
-    forall (mem : MemState) (ptr : addr) (t : dtyp), err uvalue.
+    forall {M} `{MemMonad MemState Provenance M} (ptr : addr) (t : dtyp), M uvalue.
 
   Parameter write :
-    forall {M : Type -> Type}
-      `{MemMonad MemState M}
+    forall {M} `{MemMonad MemState Provenance M}
       (ptr : addr) (v : uvalue) (t : dtyp),
       M unit.
 
   (** Operations for interacting with the concrete layout of memory. *)
   Parameter reserve_block : MemState -> LP.IP.intptr -> N -> option MemState.
 
-  (* TODO: Should we generalize this? *)
-  Definition MemStateT := stateT MemState.
-
   Section Handlers.
-    (* TODO: Not 100% sure of the constraints on E. *)
-
     (* TODO: Should we generalize the return type? *)
-    Parameter handle_memory : 
-      forall {E} `{FailureE -< E} `{UBE -< E} `{OOME -< E},
-        MemoryE ~> MemStateT (itree E).
+    Parameter handle_memory :
+      forall {M} `{MemMonad MemState Provenance M},
+      MemoryE ~> M.
 
     Parameter handle_intrinsic :
-      forall {E} `{FailureE -< E} `{PickE -< E} `{UBE -< E}, IntrinsicE ~> MemStateT (itree E).
+      forall {M} `{MemMonad MemState Provenance M},
+      IntrinsicE ~> M.
    End Handlers.
-
 End MemoryModel.
