src/coq/QC/GenAST.v
@@ -21,6 +21,10 @@ From ExtLib.Structures Require Export
 
 Require Import ExtLib.Data.Monads.StateMonad.
 
+Require Import List.
+
+Import ListNotations.
+
 From Vellvm Require Import LLVMAst Utilities AstLib Syntax.CFG Syntax.TypeUtil Syntax.TypToDtyp DynamicTypes Semantics.TopLevel QC.Utils.
 Require Import Integers Floats.
 
